Copied over untyped syntactic substitution for STLC

ERT/Stlc/DeBruijn/Basic.lean
@@ -1,24 +1,308 @@
 import ERT.Stlc.Basic
 import ERT.Utils.Wk
+import Mathlib.Order.MinMax
 
 namespace Stlc.DeBruijn
 
-inductive Stlc: Type
-| var (n: Nat)
-| app (s t: Stlc)
-| lam (A: Ty) (t: Stlc)
-| pair (s t: Stlc)
-| let2 (s t: Stlc)
-| cases (e l r: Stlc)
-| inl (t: Stlc)
-| inr (t: Stlc)
-| nil
-| zero
-| succ (n: Stlc)
-| natrec (n z s: Stlc)
-| abort (A: Ty)
+inductive Term (α: Type): Type
+  | var (n: Nat)
+  | app (s t: Term α)
+  | lam (A: Ty) (t: Term α)
+  | pair (s t: Term α)
+  | let2 (s t: Term α)
+  | case (e l r: Term α)
+  | inj (b: Fin 2) (t: Term α)
+  | cnst (a: α)
+  | abort (A: Ty)
 
--- TODO: weakening
+def Term.wk {α} (ρ: Nat -> Nat) : Term α -> Term α
+  | var n => var (ρ n)
+  | app s t => app (wk ρ s) (wk ρ t)
+  | lam A t => lam A (wk (liftWk ρ) t)
+  | pair s t => pair (wk ρ s) (wk ρ t)
+  | let2 s t => let2 (wk ρ s) (wk (liftWk (liftWk ρ)) t)
+  | case e l r => case (wk ρ e) (wk (liftWk ρ) l) (wk (liftWk ρ) r)
+  | inj b t => inj b (wk ρ t)
+  | t => t
+
+theorem Term.wk_id {α} (t: Term α): t.wk id = t := by
+  induction t with
+  | var _ => rfl
+  | _ => simp only [Term.wk, liftWk_id, *]
+
+theorem Term.wk_id' {α} (t: Term α): t.wk (λx => x) = t := t.wk_id
+
+theorem Term.wk_comp {α} (ρ σ: ℕ -> ℕ) (t: Term α):
+  t.wk (ρ ∘ σ) = (t.wk σ).wk ρ := by
+  induction t generalizing ρ σ with
+  | var _ => rfl
+  | _ => simp only [Term.wk, liftWk_comp, *]
+
+theorem Term.wk_lift_succ {α} (ρ: ℕ -> ℕ) (t: Term α):
+  (t.wk Nat.succ).wk (liftWk ρ) = (t.wk ρ).wk Nat.succ := by
+  rw [<-Term.wk_comp]
+  rw [liftWk_comp_succ]
+  rw [Term.wk_comp]
+
+theorem Term.wk_step_succ {α} (ρ: ℕ -> ℕ) (t: Term α):
+  (t.wk ρ).wk Nat.succ = t.wk (stepWk ρ) := by
+  rw [<-Term.wk_comp]
+  rfl
+
+def Term.fv {α}: Term α -> ℕ
+  | var n => n.succ
+  | lam _ t => t.fv.pred
+  | app s t => s.fv.max t.fv
+  | pair s t => s.fv.max t.fv
+  | let2 a e => a.fv.max e.fv.pred.pred
+  | inj _ t => t.fv
+  | case e l r => e.fv.max (l.fv.pred.max r.fv.pred)
+  | _ => 0
+
+theorem Term.wk_fv {α ρ σ} (t: Term α) (H: EqToN t.fv ρ σ): t.wk ρ = t.wk σ := by
+  induction t generalizing ρ σ with
+  | var n => exact congrArg _ (H n (Nat.le_refl n.succ))
+  | _ =>
+    simp only [Term.wk] <;>
+    simp only [Term.fv] at H
+    repeat apply congr
+    all_goals first
+      | rfl
+      | {
+        apply_assumption
+        repeat apply liftWk_eqToN_pred
+        apply H.le_sub
+        simp [le_max_iff, le_refl, true_or]
+      }
+
+theorem Term.wk_closed {α ρ} (t: Term α) (H: t.fv = 0): t.wk ρ = t :=
+  (t.wk_fv (H.symm ▸ (EqToN.zero_app _ id))).trans t.wk_id
+
+def Subst (α: Type) := ℕ -> Term α
+
+def Subst.id (α: Type): Subst α := Term.var
+
+def Subst.lift {α} (σ: Subst α): Subst α
+  | 0 => Term.var 0
+  | n+1 => (σ n).wk Nat.succ
+
+def Subst.liftn {α} (n: ℕ) (σ: Subst α): Subst α
+  | m => if m < n then Term.var m else (σ (m - n)).wk (λv => v + n)
+
+def Subst.liftn_zero {α} (σ: Subst α): σ.liftn 0 = σ := by
+  funext n
+  simp only [liftn]
+  split
+  . rename_i H; cases H
+  . exact (σ n).wk_id
+def Subst.liftn_succ {α} (n) (σ: Subst α): σ.liftn n.succ = (σ.liftn n).lift := by
+  induction n with
+  | zero =>
+    funext m
+    simp only [lift]
+    split
+    . rfl
+    . simp only [liftn]
+      split
+      . rename_i H; simp_arith at H
+      . simp_arith [Term.wk_id']
+  | succ n I =>
+    funext m
+    rw [I]
+    simp only [lift]
+    split
+    . rfl
+    . simp only [liftn]
+      split
+      . split
+        . rfl
+        . split
+          . rfl
+          . rename_i H C; exact (C (Nat.lt_of_succ_lt_succ (Nat.lt_of_succ_lt_succ H))).elim
+      . split
+        . rename_i H; simp_arith at H
+        . split
+          . rename_i C H; exact (C (Nat.succ_lt_succ (Nat.succ_lt_succ H))).elim
+          . simp only [<-Term.wk_comp]
+            apply congr
+            apply congrArg
+            funext v
+            simp_arith
+            simp_arith
+
+def Subst.liftn_eq_iterate_lift {α} (n: ℕ) (σ: Subst α): σ.liftn n = (Subst.lift^[n] σ) := by
+  induction n with
+  | zero => exact σ.liftn_zero
+  | succ n I => simp only [Function.iterate_succ_apply', Subst.liftn_succ, *]
+
+def Subst.lift_zero {α} (σ: Subst α): σ.lift 0 = Term.var 0 := rfl
+def Subst.lift_succ {α} (σ: Subst α) (n): (σ.lift n.succ) = (σ n).wk Nat.succ := rfl
+
+def Subst.lift_id (α): (id α).lift = id α := by funext n; cases n <;> rfl
+
+def Term.subst {α} (σ: Subst α): Term α -> Term α
+  | var n => σ n
+  | app s t => app (subst σ s) (subst σ t)
+  | lam A t => lam A (subst σ.lift t)
+  | pair s t => pair (subst σ s) (subst σ t)
+  | let2 a e => let2 (subst σ a) (subst σ.lift.lift e)
+  | inj b t => inj b (subst σ t)
+  | case e l r => case (subst σ e) (subst σ.lift l) (subst σ.lift r)
+  | t => t
+
+def Term.subst_id {α} (t: Term α): t.subst (Subst.id α) = t := by
+  induction t with
+  | var _ => rfl
+  | _ => simp only [Term.subst, Subst.lift_id, *]
+
+
+
+def Subst.fromWk (α) (ρ: ℕ -> ℕ): Subst α := Term.var ∘ ρ
+
+theorem Subst.fromWk_lift (α ρ): (fromWk α ρ).lift = fromWk α (liftWk ρ) := by
+  funext n; cases n <;> rfl
+
+theorem Term.subst_wk {α} (ρ: ℕ -> ℕ) (t: Term α): t.subst (Subst.fromWk α ρ) = t.wk ρ := by
+  induction t generalizing ρ with
+  | var n => rfl
+  | _ => simp only [Term.subst, Term.wk, Subst.fromWk_lift, *]
+
+theorem Term.subst_liftWkn {α} (t: Term α) (σ: Subst α) (n)
+  : (t.wk (liftWk^[n] Nat.succ)).subst (Subst.lift^[n + 1] σ)
+  = (t.subst (Subst.lift^[n] σ)).wk (liftWk^[n] Nat.succ) := by
+  induction t generalizing σ n with
+  | var v =>
+    simp only [
+      <-liftnWk_eq_iterate_liftWk,
+      <-Subst.liftn_eq_iterate_lift,
+      wk, subst, liftnWk, Subst.liftn
+    ]
+    split
+    . split
+      . simp [wk, liftnWk, *]
+      . rename_i H C; exact (C (Nat.le_step H)).elim
+    . rename_i C
+      simp_arith only [ite_false, <-wk_comp]
+      apply congr
+      . apply congrArg
+        funext v
+        simp_arith [Function.comp_apply, liftnWk]
+      . simp [Nat.succ_add, Nat.succ_sub_succ, Nat.add_sub_assoc]
+  | _ => simp only [Term.subst, Term.wk, <-Function.iterate_succ_apply', *]
+
+theorem Term.subst_lift {α} (t: Term α) (σ: Subst α)
+  : (t.wk Nat.succ).subst (σ.lift) = (t.subst σ).wk Nat.succ := t.subst_liftWkn σ 0
+
+def Subst.comp {α} (σ τ: Subst α): Subst α
+  | n => (τ n).subst σ
+
+theorem Subst.lift_comp {α} (σ τ: Subst α): (σ.comp τ).lift = σ.lift.comp τ.lift := by
+  funext n
+  cases n with
+  | zero => rfl
+  | succ n => simp [lift, comp, Term.subst_lift]
+
+theorem Term.subst_comp {α} (σ τ: Subst α) (t: Term α)
+  : t.subst (σ.comp τ) = (t.subst τ).subst σ := by
+  induction t generalizing σ τ with
+  | var n => rfl
+  | _ => simp only [Term.subst, Subst.lift_comp, *]
+
+theorem Subst.lift_eqToN_succ {α} {σ τ: Subst α} {n} (H: EqToN n σ τ): EqToN n.succ σ.lift τ.lift
+  | 0, _ => rfl
+  | m + 1, Hm => congrArg _ (H m (Nat.lt_of_succ_lt_succ Hm))
+
+theorem Subst.lift_congr_eqToN {α} {σ τ: Subst α} {n} (H: EqToN n σ τ)
+  : EqToN n σ.lift τ.lift := (lift_eqToN_succ H).succ_sub
+
+theorem Subst.lift_eqToN_pred {α} {σ τ: Subst α} {n}: EqToN n.pred σ τ -> EqToN n σ.lift τ.lift :=
+  match n with | 0 => lift_congr_eqToN | _ + 1 => lift_eqToN_succ
+
+theorem Term.subst_fv {α σ τ} (t: Term α) (H: EqToN t.fv σ τ): t.subst σ = t.subst τ := by
+  induction t generalizing σ τ with
+  | var n =>  exact H n (Nat.le_refl n.succ)
+  | _ =>
+    simp only [Term.subst] <;>
+    simp only [Term.fv] at H
+    repeat apply congr
+    all_goals first
+      | rfl
+      | {
+        apply_assumption
+        repeat apply Subst.lift_eqToN_pred
+        apply H.le_sub
+        simp [le_max_iff, le_refl, true_or]
+      }
+
+theorem Term.subst_closed {α σ} (t: Term α) (H: t.fv = 0): t.subst σ = t :=
+  (t.subst_fv (H.symm ▸ (EqToN.zero_app _ _))).trans t.subst_id
+
+def Term.subst0 {α} (t: Term α): Subst α
+  | 0 => t
+  | n + 1 => var n
+
+def Term.alpha0 {α} (t: Term α): Subst α
+  | 0 => t
+  | n => var n
+
+theorem Term.subst0_liftn_liftWk_liftn {α} (t: Term α) (ρ: ℕ -> ℕ) (s: Term α) (n)
+  : (t.wk (liftWk^[n + 1] ρ)).subst (Subst.lift^[n] (s.wk ρ).subst0)
+  = (t.subst (Subst.lift^[n] s.subst0)).wk (liftWk^[n] ρ) := by
+  induction t generalizing ρ s n with
+  | var v =>
+    simp only [
+      subst, wk,
+      <-Subst.liftn_eq_iterate_lift,
+      <-liftnWk_eq_iterate_liftWk,
+      Subst.liftn, liftnWk
+    ]
+    split
+    . split
+      . simp_arith [wk, liftnWk, *]
+      . rename_i H C
+        have H: v = n := by
+          cases H
+          rfl
+          contradiction
+        cases H
+        simp only [subst0, Nat.sub_self, ←wk_comp]
+        congr
+        funext _
+        simp [liftnWk]
+        split <;> simp_arith at *
+    . split
+      . simp_arith at *
+      . split
+        . rename_i C _ H
+          exact (C (Nat.lt_succ_of_lt H)).elim
+        . simp only [subst0]
+          split
+          . rename_i H _ _ He
+            have He := Nat.le_of_sub_eq_zero He
+            have He' := not_lt_of_le He
+            cases Nat.eq_or_lt_of_not_lt H with
+            | inl H => cases H
+            | inr H => contradiction
+          . rename_i Hv H _ _ _ He
+            cases Nat.eq_or_lt_of_not_lt H with
+            | inl H => cases H
+            | inr H =>
+              split
+              . rename_i He
+                exact (Hv (Nat.lt_succ_of_le (Nat.le_of_sub_eq_zero He))).elim
+              . simp_arith only [wk, liftnWk, Nat.add_sub_cancel, var.injEq, ite_false]
+                rw [Nat.add_sub_assoc (Nat.le_succ _)] at He
+                rw [Nat.succ_sub] at He
+                rw [Nat.sub_self] at He
+                cases He
+                rw [Nat.sub_succ, Nat.add]
+                simp_arith [*]
+                exact le_refl _
+  | _ => simp only [subst, wk, <-Function.iterate_succ_apply', *]
+
+theorem Term.subst0_liftWk {α} (t: Term α) (ρ: ℕ -> ℕ) (s: Term α)
+  : (t.wk (liftWk ρ)).subst (s.wk ρ).subst0 = (t.subst s.subst0).wk ρ :=
+  subst0_liftn_liftWk_liftn t ρ s 0
 
 -- TODO: just make this a prop or smt...
 
