ERT/Higher/Basic.lean
@@ -1,7 +1,5 @@
 import ERT.Utils.Wk
 import Mathlib.Order.MinMax
-import Std.Tactic.SolveByElim
-import Aesop
 
 namespace HERT
 
